towards strong normalization

STLC/STLC_normalization.v
@@ -1,24 +1,171 @@
 Add LoadPath "metatheory".
 Require Export STLC_soundness.
-Require Import Ensembles.
 
-Definition sn e := Acc red1 e.
+Inductive sn (e : term) : Prop :=
+| sn_intro : lc_term e → (forall e', e ⇝ e' → sn e') → sn e.
+
+Axiom c : termvar.
+Axiom wfterm_c : forall Γ τ, wfterm Γ (term_var_f c) τ.
 
 Inductive neutral : term → Prop :=
 | neutral_var : forall x, neutral (term_var_f x)
 | neutral_app : forall e e', neutral (term_app e e').
+Hint Constructors neutral.
 
-Fixpoint reduce τ : Ensemble term := match τ with
-| typ_base => 
+Fixpoint reduce Γ e τ : Prop := match τ with
+| typ_base => wfterm Γ e typ_base ∧ sn e
+| typ_arrow τ₁ τ₂ =>
+  wfterm Γ e (typ_arrow τ₁ τ₂) ∧
+  forall e', reduce Γ e' τ₁ → reduce Γ (term_app e e') τ₂
+end.
 
-Inductive reduce (e: term) : typ → Prop :=
-| reduce_base : forall Γ,
-  wfterm Γ e typ_base → sn e ->
-  reduce e typ_base
-| reduce_arrow : forall Γ τ₁ τ₂,
-  wfterm Γ e (typ_arrow τ₁ τ₂) ->
-  (forall e', reduce e' τ₁ → reduce (term_app e e') τ₂) →
-  reduce e (typ_arrow τ₁ τ₂).
+Lemma reduce_wfterm : forall τ Γ e,
+  reduce Γ e τ → wfterm Γ e τ.
+Proof.
+intro τ; induction τ; intros; simpl reduce in *; intuition auto.
+Qed.
+Hint Resolve reduce_wfterm.
 
+(*
+Lemma reduce_fv : forall τ Γ e,
+  reduce Γ e τ → fv_term e [<=] dom Γ.
+Proof.
+intros τ; induction τ; intros; simpl in *; destruct H.
+eauto using wfterm_fv.
+Admitted.
+*)
+(*
+Lemma reduce_weakening_aux : forall τ Γ₁ Γ₂ e,
+  reduce Γ₂ e τ →
+  uniq (Γ₁ ++ Γ₂) →
+  reduce (Γ₁ ++ Γ₂) e τ.
+Proof.
+intro τ; induction τ; intros; simpl reduce in *; destruct H; split; auto.
+apply wfterm_weakening with (Γ₁ := nil); simpl_env; auto.
+intros.
+apply IHτ2; eauto.
+*)
+
+(*
+Lemma reduce_weakening_aux : forall τ Γ e x τ',
+  ((reduce Γ e τ ∧ x ∉ dom Γ) ↔
+    (reduce (x ~ τ' ++ Γ) e τ ∧ x ∉ fv_term e)).
+Proof.
+intro τ; induction τ; intros; split; intro H; simpl reduce in *; decompose record H; clear H; split; try split; intros; simpl_env in *; eauto.
+Case "typ_base".
+apply wfterm_weakening with (Γ₁ := nil); simpl_env; eauto.
+assert (fv_term e [<=] dom Γ) by eauto using wfterm_fv; auto.
+eapply wfterm_strengthening with (Γ₁ := nil); simpl_env; eauto.
+assert (uniq (x ~ τ' ++ Γ)) by eauto; solve_uniq.
+Case "typ_arrow".
+
+
+
+simpl in H; rewrite <- IHτ1 in H; auto.
+Focus 2.
+apply H1 in H2. rewrite IHτ2 in H2; simpl; auto. eauto.
+assert (fv_term (term_app e e') [<=] dom Γ) by eauto using reduce_fv.
+simpl in H3. auto.
+
+solve_uniq.
+*)
+
+Lemma sn_regular : forall e, sn e → lc_term e.
+Proof.
+intros e H; destruct H; assumption.
+Qed.
+Hint Resolve sn_regular.
+
+Lemma sn_red : forall e e', sn e → e ⇝ e' → sn e'.
+Proof.
+intros e e' He Hred.
+induction He.
+auto.
+Qed.
+
+Lemma cr2 : forall Γ τ e e',
+  reduce Γ e τ → e ⇝ e' → reduce Γ e' τ.
+Proof.
+intros Γ τ e e' H1 H2.
+assert (wfterm Γ e τ) as H3 by auto using reduce_wfterm.
+assert (wfterm Γ e' τ) as H4 by eauto using subject_reduction.
+generalize dependent Γ. generalize dependent e. generalize dependent e'.
+induction τ; intros; simpl reduce in *; split; try split; intros; try tauto; eauto.
+destruct H1; eauto using sn_red.
+destruct H1. apply IHτ2 with (e := term_app e e'0); auto.
+apply red1_appL; eauto using reduce_wfterm.
+econstructor; eauto using reduce_wfterm.
+Qed.
+
+Lemma sn_appR : forall e e',
+  sn (term_app e e') → sn e.
+Proof.
+intros e e' H.
+remember (term_app e e') as f.
+generalize dependent e. generalize dependent e'.
+induction H; intros; subst.
+inversion H; subst.
+apply sn_intro; intros; eauto.
+Qed.
+
+Lemma cr1_cr3 : forall τ Γ,
+(forall e, reduce Γ e τ → sn e) ∧
+(forall e, neutral e →
+  wfterm Γ e τ →
+  (forall e', e ⇝ e' → reduce Γ e' τ) ->
+  reduce Γ e τ).
+Proof.
+intro τ; induction τ; intros; split; intros; simpl reduce in *; split; auto; intros; intuition eauto.
+Case "typ_base1".
+eauto using sn_red.
+Case "typ_base2".
+apply sn_intro; intros; [eauto | edestruct H1; eauto].
+Case "typ_arrow1".
+destruct (IHτ2 Γ) as [H21 H22]; clear IHτ2.
+assert (reduce Γ (term_var_f c) τ1).
+  destruct (IHτ1 Γ); apply H3; eauto using wfterm_c; intros;
+  inversion H4; subst; inversion H5.
+apply sn_red with (e := e); auto.
+apply (sn_appR _ (term_var_f c)); eauto.
+Case "typ_arrow2".
+destruct (IHτ1 Γ) as [H11 H12]; clear IHτ1.
+destruct (IHτ2 Γ) as [H21 H22]; clear IHτ2.
+assert (sn e') as H3 by auto.
+induction H3.
+eapply H22; eauto using reduce_wfterm; intros.
+inversion H6; subst.
+inversion H7; subst; inversion H.
+edestruct H1 as [_ H8]; eauto.
+eauto using cr2.
+Qed.
+
+Lemma cr1 :  forall τ Γ e, reduce Γ e τ → sn e.
+Proof.
+intros τ Γ; destruct (cr1_cr3 τ Γ); auto.
+Qed.
+
+Lemma cr3 : forall τ Γ e,
+  neutral e →
+  wfterm Γ e τ →
+  (forall e', e ⇝ e' → reduce Γ e' τ) ->
+  reduce Γ e τ.
+Proof.
+intros τ Γ; destruct (cr1_cr3 τ Γ); auto.
+Qed.
+
+Lemma reduce_const : forall τ Γ, reduce Γ (term_var_f c) τ.
+Proof.
+intros τ Γ.
+apply cr3; auto using wfterm_c; intros.
+inversion H; subst; inversion H0.
+Qed.
+
+Theorem abs_step_reduce_lemma : forall Γ e₁ e₂ τ₁ τ₂,
+  sn e₁ -> sn (term_app e₂ (term_var_f c)) -> reduce Γ e₁ τ₁ ->
+     (forall e, reduce Γ e τ₁ -> reduce Γ (term_app e₂ e) τ₂) ->
+     wfterm Γ (term_abs τ₁ e₂) (typ_arrow τ₁ τ₂) ->
+       reduce Γ (term_app (term_abs τ₁ e₂) e₁) τ₂.
+Proof.
+ICI
 
 Theorem strong_normalization : well_founded red1.
